Semantics/Dynamic/If1.v
@@ -1,3 +1,4 @@
+From Coq Require Import ssreflect.
 From Coq Require Import String.
 
 From ExtensibleCompiler.Syntax.Terms Require Import Bool.
@@ -14,42 +15,71 @@ From ExtensibleCompiler.Theory Require Import UniversalProperty.
 
 Local Open Scope SubFunctor_scope.
 
-Definition eval__If1
-           {V} `{FunctorLaws V}
-           `{! V supports Bool}
-           `{! V supports Unit}
-           `{! V supports Stuck}
-  : forall {T}, MixinAlgebra If1 T (EvalResult V)
-  := fun _ rec '(MkIf1 condition thenBranch) env =>
-       match project__F (rec condition env) with
-       | Some (MkBool b) =>
-         if b
-         then rec thenBranch env
-         else unit
-       | None => stuck "The condition of a unary branch did not evaluate to a boolean value"
-       end.
+Section If1.
 
-Global Instance Eval__If1
-       {V} `{FunctorLaws V}
-       `{! V supports Bool}
-       `{! V supports Unit}
-       `{! V supports Stuck}
-  : forall {T}, ProgramAlgebra Eval If1 T (EvalResult V)
-  := fun T => {| programAlgebra := eval__If1; |}.
+  (*
+To evaluate an [If1], the language must have [Bool] values, which is what we
+would expect the condition to evaluate down to.  It must also have a [Unit]
+value, which should be the type of the branch.  Finally, it must have a [Stuck]
+placeholder, for when the condition does not evaluate to a boolean value.
+   *)
+  Context
+    {V}
+    `{FunctorLaws V}
+    `{! V supports Bool}
+    `{! V supports Unit}
+    `{! V supports Stuck}
+  .
 
-Inductive EvalP__If1 {E V}
-          `{FunctorLaws E} `{FunctorLaws V}
-          `{! E supports If1}
-          `{! V supports Bool}
-          `{! V supports Unit}
-          (EvalP__E : (WellFormedValue E * WellFormedValue V) -> Prop)
-  : (WellFormedValue E * WellFormedValue V) -> Prop
-  :=
-  | If1True : forall c t t',
-      EvalP__E (c, boolean true) ->
-      EvalP__E (t, t') ->
-      EvalP__If1 EvalP__E (if1 c t, t')
-  | If1alse : forall c t,
-      EvalP__E (c, boolean false) ->
-      EvalP__If1 EvalP__E (if1 c t, unit)
-.
+  Definition eval__If1
+    : forall {T}, MixinAlgebra If1 T (EvalResult V)
+    := fun _ rec '(MkIf1 condition thenBranch) env =>
+         match project__F (rec condition env) with
+         | Some (MkBool b) =>
+           if b
+           then rec thenBranch env
+           else unit
+         | None => stuck "The condition of a unary branch did not evaluate to a boolean value"
+         end.
+
+  Global Instance Eval__If1
+    : forall {T}, ProgramAlgebra ForEval If1 T (EvalResult V)
+    := fun T => {| programAlgebra := eval__If1; |}.
+
+  (* Copy of [Eval__If1] for when you need to pass [T] explicitly *)
+  Definition Eval__If1'
+    : forall T, ProgramAlgebra ForEval If1 T (EvalResult V)
+    := fun _ => Eval__If1.
+
+  Global Instance WF_Eval__If1
+    : WellFormedMendlerAlgebra Eval__If1'.
+  Proof.
+    constructor.
+    move => T T' f rec [] //.
+  Qed.
+
+  (*
+We now define an extensible big-step semantics relation [EvalRelation] that
+captures how [If1] evaluates in a larger language [E].
+   *)
+
+  Context
+    {E}
+    `{FunctorLaws E}
+    `{! E supports If1}
+  .
+
+  Inductive EvalRelation__If1
+            (EvalRelation__E : (WellFormedValue E * WellFormedValue V) -> Prop)
+    : (WellFormedValue E * WellFormedValue V) -> Prop
+    :=
+    | If1True : forall c t t',
+        EvalRelation__E (c, boolean true) ->
+        EvalRelation__E (t, t') ->
+        EvalRelation__If1 EvalRelation__E (if1 c t, t')
+    | If1alse : forall c t,
+        EvalRelation__E (c, boolean false) ->
+        EvalRelation__If1 EvalRelation__E (if1 c t, unit)
+  .
+
+End If1.
