Semantics/Dynamic/If2.v
@@ -1,4 +1,9 @@
+From Coq Require Import ssreflect.
 From Coq Require Import String.
+
+From ExtensibleCompiler.Semantics.Static Require Import If2.
+
+From ExtensibleCompiler.Syntax.Types Require Import BoolType.
 
 From ExtensibleCompiler.Syntax.Terms Require Import Bool.
 From ExtensibleCompiler.Syntax.Terms Require Import If2.
@@ -7,47 +12,203 @@ From ExtensibleCompiler.Syntax.Terms Require Import Stuck.
 From ExtensibleCompiler.Theory Require Import Algebra.
 From ExtensibleCompiler.Theory Require Import Eval.
 From ExtensibleCompiler.Theory Require Import Functor.
+From ExtensibleCompiler.Theory Require Import IndexedAlgebra.
+From ExtensibleCompiler.Theory Require Import IndexedFunctor.
+From ExtensibleCompiler.Theory Require Import IndexedSubFunctor.
 From ExtensibleCompiler.Theory Require Import ProgramAlgebra.
+From ExtensibleCompiler.Theory Require Import ProofAlgebra.
 From ExtensibleCompiler.Theory Require Import SubFunctor.
+From ExtensibleCompiler.Theory Require Import Types.
+From ExtensibleCompiler.Theory Require Import TypeSoundness.
 From ExtensibleCompiler.Theory Require Import UniversalProperty.
 
 Local Open Scope SubFunctor_scope.
 
-Definition eval__If2
-           {V} `{FunctorLaws V}
-           `{! V supports Bool}
-           `{! V supports Stuck}
-  : forall {T}, MixinAlgebra If2 T (EvalResult V)
-  := fun _ rec '(MkIf2 condition thenBranch elseBranch) env =>
-       match project__F (rec condition env) with
-       | Some (MkBool b) =>
-         if b
-         then rec thenBranch env
-         else rec elseBranch env
-       | None => stuck "The condition of a binary branch was not a boolean"
-       end.
+Section If2.
 
-Global Instance Eval__If2
-       {V} `{FunctorLaws V}
-       `{! V supports Bool}
-       `{! V supports Stuck}
-  : forall {T}, ProgramAlgebra Eval If2 T (EvalResult V)
-  := fun _ => {| programAlgebra := eval__If2; |}.
+  Context
+    {V}
+    `{FunctorLaws V}
+    `{! V supports Bool}
+    `{! V supports Stuck}
+  .
 
-Inductive EvalP__If2
-          {E V}
-          `{FunctorLaws E} `{FunctorLaws V}
-          `{! E supports If2}
-          `{! V supports Bool}
-          (EvalP__E : (WellFormedValue E * WellFormedValue V) -> Prop)
-  : (WellFormedValue E * WellFormedValue V) -> Prop
-  :=
-  | If2True : forall c t e t',
-      EvalP__E (c, boolean true) ->
-      EvalP__E (t, t') ->
-      EvalP__If2 EvalP__E (if2 c t e, t')
-  | If2False : forall c t e e',
-      EvalP__E (c, boolean false) ->
-      EvalP__E (e, e') ->
-      EvalP__If2 EvalP__E (if2 c t e, e')
-.
+  Definition eval__If2
+    : forall {T}, MixinAlgebra If2 T (EvalResult V)
+    := fun _ rec '(MkIf2 condition thenBranch elseBranch) env =>
+         match project__F (rec condition env) with
+         | Some (MkBool b) =>
+           if b
+           then rec thenBranch env
+           else rec elseBranch env
+         | None => stuck "The condition of a binary branch was not a boolean"
+         end.
+
+  Global Instance Eval__If2
+    : forall {T}, ProgramAlgebra ForEval If2 T (EvalResult V)
+    := fun _ => {| programAlgebra := eval__If2; |}.
+
+  Definition Eval__If2'
+    : forall T, ProgramAlgebra ForEval If2 T (EvalResult V)
+    := fun _ => Eval__If2.
+
+  Global Instance WellFormedMendlerAlgebra_Eval__If2
+    : WellFormedMendlerAlgebra Eval__If2'.
+  Proof.
+    constructor.
+    move => T T' f rec [] //.
+  Qed.
+
+  Context
+    {T}
+    `{FunctorLaws T}
+    `{! T supports BoolType}
+
+    {E}
+    `{FunctorLaws E}
+    `{! E supports If2}
+    `{! WellFormedSubFunctor If2 E}
+
+    `{! V supports If2}
+
+    {typeEqualityForT : forall R, ProgramAlgebra ForTypeEquality T R (TypeEqualityResult T)}
+  .
+
+  Lemma Soundness__if2
+
+        (WT : (TypedExpr T V)-indexedPropFunctor)
+        `(IndexedFunctor (TypedExpr T V) WT)
+        (* `(IndexedFunctor (TypedExpr T V) WellTyped__If2) *)
+        `((WellTyped__If2 <= WT)%IndexedSubFunctor)
+
+        `{Eval__E   : forall {R}, ProgramAlgebra ForEval   E R (EvalResult   V)}
+        `{! forall {R}, WellFormedProgramAlgebra Eval__If2 Eval__E (T := R)}
+
+        (Eval__R : Set)
+        {F} `{FunctorLaws F} `{F supports If2}
+        `{Eval__V : ProgramAlgebra ForEval F (EvalResult V) Eval__R}
+        `{! forall {R}, WellFormedProgramAlgebra Eval__If2 Eval__E (T := R)}
+        recEval
+
+        (TypeOf__R : Set)
+        `{TypeOf__E : forall {R}, ProgramAlgebra ForTypeOf E R (TypeOfResult T)}
+        `{! forall {R}, WellFormedProgramAlgebra TypeOf__If2 TypeOf__E (T := R)}
+        recTypeOf
+
+    : forall Gamma (c t e : TypeOf__R) (c' t' e' : Eval__R),
+
+      (forall tau,
+          recTypeOf c = Some tau ->
+          WellTyped__If2 (IndexedFix WT) {| type := tau; expr := (recEval c' Gamma) |}
+      ) ->
+
+      (forall tau,
+          recTypeOf t = Some tau ->
+          WellTyped__If2 (IndexedFix WT) {| type := tau; expr := (recEval t' Gamma) |}
+      ) ->
+
+      (forall tau,
+          recTypeOf e = Some tau ->
+          WellTyped__If2 (IndexedFix WT) {| type := tau; expr := (recEval e' Gamma) |}
+      ) ->
+
+      forall tau,
+        typeOf__If2 (R := TypeOf__R) recTypeOf (MkIf2 c t e) = Some tau ->
+        WellTyped__If2
+          (IndexedFix WT)
+          {|
+            type := tau;
+            expr := eval__If2 (T := Eval__R) recEval (MkIf2 c' t' e') Gamma;
+          |}.
+  Proof.
+    rewrite /=.
+    move => Gamma c t e c' t' e'.
+    case : (recTypeOf c) => // tau__c H__c.
+    move : H__c (H__c tau__c eq_refl) => _ WT__c.
+    case : (isBoolType (proj1_sig tau__c)) => //.
+    case : (recTypeOf t) => // tau__t H__t.
+    move : H__t (H__t tau__t eq_refl) => _ WT__t.
+    case : (recTypeOf e) => // tau__e H__e.
+    move : H__e (H__e tau__e eq_refl) => _ WT__e.
+    move => tau.
+    case TE : (typeEquality (proj1_sig tau__t) tau__e) => //.
+    move => [] <-.
+
+    (* TODO: implement typeEqualityCorrectness for all types *)
+
+    (* pose proof (typeEqualityCorrectness tau__t tau__e). *)
+    (* eapply typeEqualityCorrectness in TE. *)
+
+  Admitted.
+
+  Global Instance Soundness__If2
+
+         (WT : (TypedExpr T V)-indexedPropFunctor)
+         `(IndexedFunctor (TypedExpr T V) WT)
+         (* `(IndexedFunctor (TypedExpr T V) WellTyped__If2) *)
+         `((WellTyped__If2 <= WT)%IndexedSubFunctor)
+
+         `{Eval__E   : forall {R}, ProgramAlgebra ForEval   E R (EvalResult   V)}
+         `{! forall {R}, WellFormedProgramAlgebra Eval__If2 Eval__E (T := R)}
+         (recEval   : UniversalPropertyF E -> EvalResult   V)
+
+         `{TypeOf__E : forall {R}, ProgramAlgebra ForTypeOf E R (TypeOfResult T)}
+         `{! forall {R}, WellFormedProgramAlgebra TypeOf__If2 TypeOf__E (T := R)}
+         (recTypeOf : UniversalPropertyF E -> TypeOfResult T)
+
+    : ProofAlgebra
+        ForSoundness If2
+        (sig (UniversalPropertyP2
+                (AbstractSoundnessStatement' WT recEval recTypeOf))).
+  Proof.
+    constructor.
+    apply Induction2Algebra__If2.
+    rewrite / AbstractSoundnessStatement' / AbstractSoundnessStatement.
+    rewrite / UniversalPropertyP2 /=.
+    move => c t e H__c H__t H__e.
+    (* )[[UP'__c1 UP'__c2] IH__c] [[UP'__t1 UP'__t2] IH__t] [[UP'__e1 UP'__e2] IH__e] /=. *)
+    constructor.
+    {
+      apply conj; apply (proj2_sig (if2 _ _ _)).
+    }
+    {
+      move => Gamma.
+      rewrite / if2__F / if2 / inject /=.
+      repeat rewrite unwrap__UP'_wrap__F /=.
+      repeat rewrite fmapFusion /=.
+      rewrite / Extras.compose /=.
+      repeat rewrite wellFormedSubFunctor => //=.
+      rewrite / programAlgebra'.
+      repeat rewrite wellFormedProgramAlgebra.
+      move => IH tau TY.
+      apply (iInject (F := WellTyped__If2)).
+
+      (* econstructor. *)
+      (* move : TY. *)
+      (* rewrite {1} / programAlgebra. *)
+      (* move : (IH__e Gamma). *)
+      (* constructor. *)
+      (* rewrite / project__F /=. *)
+      (* econstructor => //. *)
+      (* move : c H__c TY => [a b] H__ab TY /=. *)
+      (* move : TY => /=. *)
+      (* move => [] <- //. *)
+
+
+  Admitted.
+
+  Inductive EvalRelation__If2
+            (EvalRelation__E : (WellFormedValue E * WellFormedValue V) -> Prop)
+    : (WellFormedValue E * WellFormedValue V) -> Prop
+    :=
+    | If2True : forall c t e t',
+        EvalRelation__E (c, boolean true) ->
+        EvalRelation__E (t, t') ->
+        EvalRelation__If2 EvalRelation__E (if2 c t e, t')
+    | If2False : forall c t e e',
+        EvalRelation__E (c, boolean false) ->
+        EvalRelation__E (e, e') ->
+        EvalRelation__If2 EvalRelation__E (if2 c t e, e')
+  .
+
+End If2.
