Semantics/Dynamic/Unit.v
@@ -1,35 +1,209 @@
+From Coq Require Import ssreflect.
 From Coq Require Import String.
+
+From ExtensibleCompiler.Semantics.Static Require Import Unit.
 
 From ExtensibleCompiler.Syntax.Terms Require Import Unit.
 
+From ExtensibleCompiler.Syntax.Types Require Import UnitType.
+
 From ExtensibleCompiler.Theory Require Import Algebra.
 From ExtensibleCompiler.Theory Require Import Eval.
-From ExtensibleCompiler.Theory Require Import Functor.
-From ExtensibleCompiler.Theory Require Import ProgramAlgebra.
 From ExtensibleCompiler.Theory Require Import SubFunctor.
+From ExtensibleCompiler.Theory Require Import Functor.
+From ExtensibleCompiler.Theory Require Import IndexedAlgebra.
+From ExtensibleCompiler.Theory Require Import IndexedFunctor.
+From ExtensibleCompiler.Theory Require Import IndexedSubFunctor.
+From ExtensibleCompiler.Theory Require Import ProofAlgebra.
+From ExtensibleCompiler.Theory Require Import ProgramAlgebra.
+From ExtensibleCompiler.Theory Require Import Types.
+From ExtensibleCompiler.Theory Require Import TypeSoundness.
 From ExtensibleCompiler.Theory Require Import UniversalProperty.
 
 Local Open Scope SubFunctor_scope.
 
-Definition eval__Unit
-           {V} `{FunctorLaws V}
-           `{! V supports Unit}
-  : forall {T}, MixinAlgebra Unit T (EvalResult V)
-  := fun T rec '(MkUnit) env => unit.
+Section AbstractLemma.
 
-Global Instance Eval__Unit
-       {V} `{FunctorLaws V}
-       `{! V supports Unit}
-  : forall {T}, ProgramAlgebra Eval Unit T (EvalResult V)
-  := fun T => {| programAlgebra := eval__Unit; |}.
+  Context
+    {T}
+    `{FunctorLaws T}
+    {C}
+    `{FunctorLaws C}
+    {E}
+    `{FunctorLaws E}
+    `{! E supports C}
+    `{! WellFormedSubFunctor C E}
+    {V}
+    `{FunctorLaws V}
+  .
 
-Inductive EvalP__Unit
-          {L V}
-          `{FunctorLaws L} `{FunctorLaws V}
-          `{! L supports Unit}
-          `{! V supports Unit}
-          (EvalP__E : (WellFormedValue L * WellFormedValue V) -> Prop)
-  : (WellFormedValue L * WellFormedValue V) -> Prop
-  :=
-  | UnitValue : EvalP__Unit EvalP__E (unit, unit)
-.
+  Theorem EvenMoreAbstractSoundness
+         (WT__C : (TypedExpr T V)-indexedPropFunctor)
+         (WT__E : (TypedExpr T V)-indexedPropFunctor)
+         `(IndexedFunctor (TypedExpr T V) WT__C)
+         `(IndexedFunctor (TypedExpr T V) WT__E)
+         `(! IndexedSubFunctor WT__C WT__E)
+
+         `{Eval__C   : forall {R}, ProgramAlgebra ForEval   C R (EvalResult   V)}
+         `{Eval__E   : forall {R}, ProgramAlgebra ForEval   E R (EvalResult   V)}
+         `{! forall {R}, WellFormedProgramAlgebra Eval__C Eval__E (T := R)}
+         (recEval   : UniversalPropertyF E -> EvalResult   V)
+
+         `{TypeOf__C : forall {R}, ProgramAlgebra ForTypeOf C R (TypeOfResult T)}
+         `{TypeOf__E : forall {R}, ProgramAlgebra ForTypeOf E R (TypeOfResult T)}
+         `{! forall {R}, WellFormedProgramAlgebra TypeOf__C TypeOf__E (T := R)}
+         (recTypeOf : UniversalPropertyF E -> TypeOfResult T)
+
+         Gamma (ctor : C (WellFormedValue E))
+
+    :
+      (forall
+          (Gamma' : Environment.Environment (ValueFix V))
+          (a : UniversalPropertyF E * UniversalPropertyF E),
+          (forall tau : TypeFix T,
+              programAlgebra' TypeOf__E recTypeOf (unwrap__UP' (proj1_sig (snd a))) =
+              Some tau ->
+              WellTyped WT__E tau
+                        (programAlgebra' Eval__E recEval (unwrap__UP' (proj1_sig (fst a)))
+                                         Gamma')) ->
+          forall tau : TypeFix T,
+            recTypeOf (snd a) = Some tau ->
+            WellTyped WT__E tau (recEval (wrap__UP' (unwrap__UP' (proj1_sig (fst a)))) Gamma')) ->
+      forall tau : TypeFix T,
+        programAlgebra' TypeOf__E recTypeOf (unwrap__UP' (proj1_sig (inject ctor))) = Some tau ->
+
+        (WT__C (IndexedFix WT__E) ({|
+             type := tau;
+             expr := programAlgebra' Eval__E recEval (unwrap__UP' (proj1_sig (inject ctor))) Gamma;
+           |})) ->
+
+
+        WellTyped WT__E tau
+                  (programAlgebra' Eval__E recEval (unwrap__UP' (proj1_sig (inject ctor))) Gamma).
+  Proof.
+    rewrite / inject /=.
+    rewrite unwrap__UP'_wrap__F /=.
+    rewrite fmapFusion / Extras.compose /=.
+    rewrite wellFormedSubFunctor => //=.
+    rewrite / programAlgebra'.
+    rewrite wellFormedProgramAlgebra.
+    rewrite wellFormedProgramAlgebra.
+    move => IH tau TY.
+    apply (iInject (F := WT__C)) => /=.
+  Qed.
+
+End AbstractLemma.
+
+Section Unit.
+
+  Context
+    {V}
+    `{FunctorLaws V}
+    `{! V supports Unit}
+    `{! WellFormedSubFunctor Unit V}
+  .
+
+  Definition eval__Unit
+    : forall {R}, MixinAlgebra Unit R (EvalResult V)
+    := fun _ rec '(MkUnit) env => unit.
+
+  Global Instance Eval__Unit
+    : forall {R}, ProgramAlgebra ForEval Unit R (EvalResult V)
+    := fun _ => {| programAlgebra := eval__Unit; |}.
+
+  Definition Eval__Unit'
+    : forall R, ProgramAlgebra ForEval Unit R (EvalResult V)
+    := fun _ => Eval__Unit.
+
+  Global Instance WF_Eval__Bool
+    : WellFormedMendlerAlgebra Eval__Unit'.
+  Proof.
+    constructor.
+    move => T T' f rec [] //.
+  Qed.
+
+  Context
+    {E}
+    `{FunctorLaws E}
+    `{! E supports Unit}
+    `{!WellFormedSubFunctor Unit E}
+  .
+
+  Inductive EvalRelation__Unit
+            (EvalRelation__E : (WellFormedValue E * WellFormedValue V) -> Prop)
+    : (WellFormedValue E * WellFormedValue V) -> Prop
+    :=
+    | UnitValue : EvalRelation__Unit EvalRelation__E (unit, unit)
+  .
+
+  Context
+    {T}
+    `{FunctorLaws T}
+    `{! T supports UnitType}
+    `{! WellFormedSubFunctor UnitType T}
+  .
+
+  Inductive WellTyped__Unit
+            (WT : (TypedExpr T V)-indexedProp)
+    : (TypedExpr T V)-indexedProp
+    :=
+    | WellTyped__unit : forall t e,
+        proj1_sig e = unit__F ->
+        proj1_sig t = unitType ->
+        WellTyped__Unit WT {| type := t; expr := e; |}
+  .
+
+  Global Instance IndexedFunctor_WellTyped__Unit
+    : IndexedFunctor (TypedExpr T V) WellTyped__Unit.
+  Proof.
+    constructor.
+    move => A B i IH [] [t UP__t] [e UP__e] /= => Eq__e Eq__t.
+    move : Eq__t Eq__e UP__t UP__e => -> -> => UP__t UP__e.
+    econstructor => //.
+  Qed.
+
+  Global Instance Soundness__Unit
+
+         (WT : (TypedExpr T V)-indexedPropFunctor)
+         `(IndexedFunctor (TypedExpr T V) WT)
+         `((WellTyped__Unit <= WT)%IndexedSubFunctor)
+
+         `{Eval__E   : forall {R}, ProgramAlgebra ForEval   E R (EvalResult   V)}
+         `{! forall {R}, WellFormedProgramAlgebra Eval__Unit Eval__E (T := R)}
+         (recEval   : UniversalPropertyF E -> EvalResult   V)
+
+         `{TypeOf__E : forall {R}, ProgramAlgebra ForTypeOf E R (TypeOfResult T)}
+         `{! forall {R}, WellFormedProgramAlgebra TypeOf__Unit TypeOf__E (T := R)}
+         (recTypeOf : UniversalPropertyF E -> TypeOfResult T)
+
+    : ProofAlgebra
+        ForSoundness Unit
+        (sig (UniversalPropertyP2
+                (AbstractSoundnessStatement' WT recEval recTypeOf))).
+  Proof.
+    constructor.
+    apply Induction2Algebra__Unit.
+    rewrite / AbstractSoundnessStatement' / AbstractSoundnessStatement.
+    rewrite / UniversalPropertyP2 /=.
+    constructor.
+    {
+      apply conj; apply (proj2_sig unit).
+    }
+    {
+      move => Gamma.
+      rewrite / unit__F / unit / inject /=.
+      rewrite unwrap__UP'_wrap__F /=.
+      rewrite fmapFusion / Extras.compose /=.
+      rewrite wellFormedSubFunctor => //=.
+      rewrite / programAlgebra'.
+      rewrite wellFormedProgramAlgebra.
+      rewrite wellFormedProgramAlgebra.
+      move => IH tau TY.
+      apply (iInject (F := WellTyped__Unit)) => /=.
+      econstructor => //.
+      move : TY => /=.
+      move => [] <- //.
+    }
+  Qed.
+
+End Unit.
