Semantics/Static/If2.v
@@ -1,37 +1,95 @@
+From Coq Require Import ssreflect.
+
 From ExtensibleCompiler.Syntax.Terms Require Import If2.
 
 From ExtensibleCompiler.Syntax.Types Require Import BoolType.
 
 From ExtensibleCompiler.Theory Require Import Algebra.
 From ExtensibleCompiler.Theory Require Import Functor.
+From ExtensibleCompiler.Theory Require Import IndexedFunctor.
 From ExtensibleCompiler.Theory Require Import ProgramAlgebra.
+From ExtensibleCompiler.Theory Require Import ProofAlgebra.
 From ExtensibleCompiler.Theory Require Import SubFunctor.
 From ExtensibleCompiler.Theory Require Import Types.
+From ExtensibleCompiler.Theory Require Import TypeSoundness.
+From ExtensibleCompiler.Theory Require Import UniversalProperty.
 
 Local Open Scope SubFunctor_scope.
 
-Definition typeOf__If2
-           {LT} `{FunctorLaws LT} `{LT supports BoolType}
-           {typeEqualityForLT : forall T, ProgramAlgebra TypeEquality LT T (TypeEqualityResult LT)}
-  : forall {T}, MixinAlgebra If2 T (TypeOfResult LT)
-  := fun _ rec '(MkIf2 c t e) =>
-       match rec c with
-       | Some cType =>
-         if isBoolType (proj1_sig cType)
-         then
-           match (rec t, rec e) with
-           | (Some tType, Some eType) =>
-             if typeEquality LT (proj1_sig tType) eType
-             then Some tType
-             else None
-           | _ => None
-           end
-         else None
-       | None => None
-       end.
+Section If2.
 
-Global Instance TypeOf__If2
-       {LT} `{FunctorLaws LT} `{LT supports BoolType}
-       {typeEqualityForLT : forall T, ProgramAlgebra TypeEquality LT T (TypeEqualityResult LT)}
-  : forall {T}, ProgramAlgebra TypeOf If2 T (TypeOfResult LT)
-  := fun _ => {| programAlgebra := typeOf__If2; |}.
+  Context
+    {T}
+    `{FunctorLaws T}
+    `{! T supports BoolType}
+    `{! WellFormedSubFunctor BoolType T}
+  .
+
+  Context
+    {typeEqualityForT : forall R, ProgramAlgebra ForTypeEquality T R (TypeEqualityResult T)}
+    (* {typeEqualityCorrectnessForT
+     : ProofAlgebra ForTypeEqualityCorrectness
+                    T (sig (UniversalPropertyP typeEqualityCorrectnessStatement))} *)
+  .
+
+  Definition typeOf__If2
+    : forall {R}, MixinAlgebra If2 R (TypeOfResult T)
+    := fun _ rec '(MkIf2 c t e) =>
+         match rec c with
+         | Some cType =>
+           if isBoolType (proj1_sig cType)
+           then
+             match (rec t, rec e) with
+             | (Some tType, Some eType) =>
+               if typeEquality (proj1_sig tType) eType
+               then Some tType
+               else None
+             | _ => None
+             end
+           else None
+         | None => None
+         end.
+
+  Global Instance TypeOf__If2
+    : forall {R}, ProgramAlgebra ForTypeOf If2 R (TypeOfResult T)
+    := fun _ => {| programAlgebra := typeOf__If2; |}.
+
+  Definition TypeOf__If2'
+    : forall R, ProgramAlgebra ForTypeOf If2 R (TypeOfResult T)
+    := fun _ => TypeOf__If2.
+
+  Global Instance WellFormedMendlerAlgebra_TypeOf__If2
+    : WellFormedMendlerAlgebra TypeOf__If2'.
+  Proof.
+    constructor.
+    move => T' T'' f rec [] //.
+  Qed.
+
+  Context
+    {E}
+    `{FunctorLaws E}
+    `{E supports If2}
+  .
+
+  Inductive WellTyped__If2
+            (WT : (TypedExpr T E)-indexedProp)
+    : (TypedExpr T E)-indexedProp
+    :=
+    | WellTyped__if2 : forall t e condition thenBranch elseBranch,
+        proj1_sig e = if2__F condition thenBranch elseBranch ->
+        WT {| type := boolType';  expr := condition; |} ->
+        WT {| type := t;          expr := thenBranch; |} ->
+        WT {| type := t;          expr := elseBranch; |} ->
+        WellTyped__If2 WT {| type := t; expr := e; |}
+  .
+
+  Global Instance IndexedFunctor_WellTyped__If2
+    : IndexedFunctor (TypedExpr T E) WellTyped__If2.
+  Proof.
+    constructor.
+    move => A B i IH [] [t UP__t] [e UP__e] /= => cond thenB elseB Eq__e.
+    move : Eq__e UP__e => -> => UP__e H__c H__t H__e.
+    econstructor => //; apply IH => //.
+  Qed.
+
+End If2.
