Test/Semantics/Dynamic.v
@@ -8,11 +8,19 @@ From ExtensibleCompiler.Semantics.Dynamic Require Import If1.
 From ExtensibleCompiler.Semantics.Dynamic Require Import If2.
 From ExtensibleCompiler.Semantics.Dynamic Require Import Unit.
 
+From ExtensibleCompiler.Semantics.Static Require Import Bool.
+From ExtensibleCompiler.Semantics.Static Require Import If1.
+From ExtensibleCompiler.Semantics.Static Require Import If2.
+From ExtensibleCompiler.Semantics.Static Require Import Unit.
+
 From ExtensibleCompiler.Syntax.Terms Require Import Bool.
 From ExtensibleCompiler.Syntax.Terms Require Import If1.
 From ExtensibleCompiler.Syntax.Terms Require Import If2.
 From ExtensibleCompiler.Syntax.Terms Require Import Stuck.
 From ExtensibleCompiler.Syntax.Terms Require Import Unit.
+
+From ExtensibleCompiler.Syntax.Types Require Import BoolType.
+From ExtensibleCompiler.Syntax.Types Require Import UnitType.
 
 From ExtensibleCompiler.Theory Require Import Algebra.
 From ExtensibleCompiler.Theory Require Import Environment.
@@ -25,19 +33,26 @@ From ExtensibleCompiler.Theory Require Import ProgramAlgebra.
 From ExtensibleCompiler.Theory Require Import ProofAlgebra.
 From ExtensibleCompiler.Theory Require Import SubFunctor.
 From ExtensibleCompiler.Theory Require Import Sum1.
+From ExtensibleCompiler.Theory Require Import Types.
+From ExtensibleCompiler.Theory Require Import TypeSoundness.
 From ExtensibleCompiler.Theory Require Import UniversalProperty.
 
 Local Open Scope Sum1_scope.
 Local Open Scope SubFunctor_scope.
 
-(* Create a language [L] that supports [Bool], [If2], and [Unit] *)
-Definition L := (Bool + If2 + Unit).
+(* Create a type language [T] *)
+Definition T := (BoolType + UnitType).
 
-(* Creates a type language [LT] that supports [Bool] and [Unit] *)
+(* Create an expression language [E] *)
+Definition E := (Bool + If2 + Unit).
+
+(* Create a value language [V] *)
 Definition V := (Bool + Stuck + Unit).
 
-(* Create a concrete representation for the result of type-checking, so
-   that it is easy to inspect manually *)
+(*
+Create a concrete representation for the result of type-checking, so that it is
+easy to inspect manually
+ *)
 Inductive Result :=
 | BoolValue (b : bool)
 | UnitValue
@@ -59,53 +74,81 @@ Global Instance computeResult
          ;
        |}.
 
-Definition eval
-           (b : WellFormedValue L)
+Definition eval'
+           (e : WellFormedValue E)
   : Result
   := foldProgramAlgebra
        (Alg := computeResult)
-       (proj1_sig (eval (L := L) (V := V) (proj1_sig b) (empty _))).
+       (proj1_sig (eval (L := E) (V := V) (proj1_sig e) (empty _))).
 
-Theorem regression__unit : eval unit = UnitValue.
+Theorem regression__unit : eval' unit = UnitValue.
 Proof. reflexivity. Qed.
 
-Theorem regression__true : eval (boolean true) = BoolValue true.
+Theorem regression__true : eval' (boolean true) = BoolValue true.
 Proof. reflexivity. Qed.
 
-Theorem regression__false : eval (boolean false) = BoolValue false.
+Theorem regression__false : eval' (boolean false) = BoolValue false.
 Proof. reflexivity. Qed.
 
 Theorem regression__if2True
-  : eval (if2 (boolean true) (boolean true) (boolean false)) = BoolValue true.
+  : eval' (if2 (boolean true) (boolean true) (boolean false)) = BoolValue true.
 Proof. reflexivity. Qed.
 
 Theorem regression__if2False
-  : eval (if2 (boolean false) (boolean true) (boolean false)) = BoolValue false.
+  : eval' (if2 (boolean false) (boolean true) (boolean false)) = BoolValue false.
 Proof. reflexivity. Qed.
 
 Theorem regression__if2IllTypedCondition
-  : eval (if2 unit (boolean true) (boolean false)) = EvalFailed.
+  : eval' (if2 unit (boolean true) (boolean false)) = EvalFailed.
 Proof. reflexivity. Qed.
 
 Theorem regression__if2IllTypedBranchStillWorksLeft
-  : eval (if2 (boolean true) (boolean true) unit) = BoolValue true.
+  : eval' (if2 (boolean true) (boolean true) unit) = BoolValue true.
 Proof. reflexivity. Qed.
 
 Theorem regression__if2IllTypedBranchStillWorksRight
-  : eval (if2 (boolean false) unit (boolean false)) = BoolValue false.
+  : eval' (if2 (boolean false) unit (boolean false)) = BoolValue false.
 Proof. reflexivity. Qed.
+
+(*
+Let's make sure that we can instantiate the statement of type soundness through
+evaluation.
+ *)
+
+Definition WellTyped__E
+  : (TypedExpr T V)-indexedPropFunctor
+  := (WellTyped__Bool).
+
+(* Algebra to turn the extensible results into concrete results *)
+
+Theorem Soundness__EvalE
+  : forall (e : WellFormedValue E) Gamma (tau : TypeFix T),
+    typeOf (proj1_sig e) = Some tau ->
+    WellTyped WellTyped__E tau (eval (proj1_sig e) Gamma).
+Proof.
+  eapply Soundness => //.
+  typeclasses eauto.
+  typeclasses eauto.
+Admitted.
+
+
+
+
+
+
+
 
 Definition SourceExpr := Bool + If1 + Unit.
 Definition TargetExpr := Bool + If2 + Unit.
 Definition Value := Bool + Stuck + Unit.
 
-Definition EvalP__Source
-  : (WellFormedValue SourceExpr * WellFormedValue Value)-indexedProp
-  := (EvalP__Bool + EvalP__If1)%IndexedSum1.
+Definition EvalRelation__Source
+  : (WellFormedValue SourceExpr * WellFormedValue Value)-indexedPropFunctor
+  := (EvalRelation__Bool + EvalRelation__If1 + EvalRelation__Unit)%IndexedSum1.
 
-Definition EvalP__Target
-  : (WellFormedValue TargetExpr * WellFormedValue Value)-indexedProp
-  := (EvalP__Bool + EvalP__If2 + EvalP__Unit)%IndexedSum1.
+Definition EvalRelation__Target
+  : (WellFormedValue TargetExpr * WellFormedValue Value)-indexedPropFunctor
+  := (EvalRelation__Bool + EvalRelation__If2 + EvalRelation__Unit)%IndexedSum1.
 
 Definition removeUnaryIfs
            (e : WellFormedValue SourceExpr)
@@ -118,12 +161,12 @@ Proof. reflexivity. Qed.
 
 Theorem removeUnaryIfsCorrectness
   : forall e v,
-    IndexedFix EvalP__Source (e, v) ->
-    IndexedFix EvalP__Target (removeUnaryIfs e, v).
+    IndexedFix EvalRelation__Source (e, v) ->
+    IndexedFix EvalRelation__Target (removeUnaryIfs e, v).
 Proof.
   move => e v S.
   pose proof (@iUnwrapFix) as U.
-  specialize (U _ EvalP__Source).
+  specialize (U _ EvalRelation__Source).
 
   (* TODO: IndexedFunctor instances *)
 
