Theory/IndexedAlgebra.v
@@ -5,37 +5,43 @@ From ExtensibleCompiler.Theory Require Import IndexedSum1.
 
 Local Open Scope IndexedSum1_scope.
 
-Definition IndexedAlgebra {I} (F : I-indexedProp) A
+Definition IndexedAlgebra
+           {I} (F : I-indexedPropFunctor) (A : I-indexedProp)
+  : Prop
   := forall i, F A i -> A i.
 
-Definition IndexedMendlerAlgebra {I} (F : I-indexedProp) (A : I -> Prop) : Prop
+Definition IndexedMendlerAlgebra
+           {I} (F : I-indexedPropFunctor) (A : I-indexedProp)
+  : Prop
   := forall i (R : I -> Prop), (forall i, R i -> A i) -> F R i -> A i.
 
-Definition IndexedFix {I} (F : I-indexedProp) i : Prop
-  := forall (A : I -> Prop), IndexedMendlerAlgebra F A -> A i.
+Definition IndexedFix
+           {I} (F : I-indexedPropFunctor) i
+  : Prop
+  := forall (A : I-indexedProp), IndexedMendlerAlgebra F A -> A i.
 
 Definition
   iMendlerFold
-  {I} {F : I-indexedProp} {A : I -> Prop} (f : IndexedMendlerAlgebra F A) i
+  {I} {F : I-indexedPropFunctor} {A : I -> Prop} (f : IndexedMendlerAlgebra F A) i
   : IndexedFix F i -> A i
   := fun e => e A f.
 
 Definition
   iWrapFix
-  {I} {F : I-indexedProp} i (unwrapped : F (IndexedFix F) i)
+  {I} {F : I-indexedPropFunctor} i (unwrapped : F (IndexedFix F) i)
   : IndexedFix F i
   := fun A f
      => f i (IndexedFix F) (iMendlerFold f) unwrapped.
 
 Definition
   ifold
-  {I} {F : I-indexedProp} `{IndexedFunctor I F} {A : I -> Prop}
+  {I} {F : I-indexedPropFunctor} `{IndexedFunctor I F} {A : I-indexedProp}
   (f : IndexedAlgebra F A) i (e : IndexedFix F i)
   : A i
   := iMendlerFold (fun i' r rec fa => f i' (indexedFmap i' rec fa)) i e.
 
 Definition
   iUnwrapFix
-  {I} {F : I-indexedProp} `{IndexedFunctor I F}
+  {I} {F : I-indexedPropFunctor} `{IndexedFunctor I F}
   : forall (i : I), IndexedFix F i -> F (IndexedFix F) i
   := ifold (fun i => indexedFmap i iWrapFix).
