Theory/IndexedSubFunctor.v
@@ -5,7 +5,7 @@ From ExtensibleCompiler.Theory Require Import IndexedSum1.
 Local Open Scope IndexedSum1_scope.
 
 Class IndexedSubFunctor
-      {I} (F G : I-indexedProp)
+      {I} (F G : I-indexedPropFunctor)
       `{IndexedFunctor I F} `{IndexedFunctor I G}
   : Prop
   :=
@@ -20,14 +20,14 @@ Local Open Scope IndexedSubFunctor_scope.
 
 Definition
   iInject
-  {I} {F G : I-indexedProp} `{IndexedFunctor I F} `{IndexedFunctor I G} `{F <= G} {i}
+  {I} {F G : I-indexedPropFunctor} `{IndexedFunctor I F} `{IndexedFunctor I G} `{F <= G} {i}
   (fexp : F (IndexedFix G) i)
   : IndexedFix G i
   := iWrapFix i (iInj fexp).
 
 Definition
   iProject
-  {I} {F G : I-indexedProp} `{IndexedFunctor I F} `{IndexedFunctor I G} `{F <= G} {i}
+  {I} {F G : I-indexedPropFunctor} `{IndexedFunctor I F} `{IndexedFunctor I G} `{F <= G} {i}
   (g : IndexedFix G i)
   : F (IndexedFix G) i \/ True
   := iPrj (iUnwrapFix i g).
