Theory/Types.v
@@ -1,6 +1,9 @@
+From Coq Require Import ssreflect.
+
 From ExtensibleCompiler.Theory Require Import Algebra.
 From ExtensibleCompiler.Theory Require Import Functor.
 From ExtensibleCompiler.Theory Require Import ProgramAlgebra.
+From ExtensibleCompiler.Theory Require Import ProofAlgebra.
 From ExtensibleCompiler.Theory Require Import UniversalProperty.
 
 (** [TypeFix] is just an alias for [UniversalPropertyF], but it makes it so that
@@ -13,12 +16,12 @@ Definition TypeOfResult
            LT `{FunctorLaws LT}
   := option (TypeFix LT).
 
-Variant TypeOf := .
+Variant ForTypeOf := .
 
 Definition typeOf
            {L LT}
            `{FunctorLaws L} `{FunctorLaws LT}
-           {TypeOfL : forall T, ProgramAlgebra TypeOf L T (TypeOfResult LT)}
+           {TypeOfL : forall T, ProgramAlgebra ForTypeOf L T (TypeOfResult LT)}
   : Fix L -> TypeOfResult LT
   := mendlerFold (fun _ => @programAlgebra _ _ _ _ _ _ (TypeOfL _)).
 
@@ -26,10 +29,47 @@ Definition TypeEqualityResult
            LT `{FunctorLaws LT}
   := TypeFix LT -> bool.
 
-Variant TypeEquality := .
+Variant ForTypeEquality := .
 
 Definition typeEquality
-           LT `{FunctorLaws LT}
-           {typeEqualityForLT : forall T, ProgramAlgebra TypeEquality LT T (TypeEqualityResult LT)}
-  : Fix LT -> TypeEqualityResult LT
-  := mendlerFold (fun _ => @programAlgebra _ _ _ _ _ _ (typeEqualityForLT _)).
+           {T} `{FunctorLaws T}
+           {typeEqualityForT :
+              forall R,
+                ProgramAlgebra ForTypeEquality T R (TypeEqualityResult T)}
+  : Fix T -> TypeEqualityResult T
+  := mendlerFold (fun _ => @programAlgebra _ _ _ _ _ _ (typeEqualityForT _)).
+
+Definition typeEqualityCorrectnessStatement
+           {T} `{FunctorLaws T}
+           {typeEqualityForT :
+              forall R,
+                ProgramAlgebra ForTypeEquality T R (TypeEqualityResult T)}
+           (tau : Fix T)
+           (UP'__tau : Fold__UP' tau)
+  : Prop
+  := forall tau',
+    typeEquality tau tau' = true ->
+    tau = proj1_sig tau'.
+
+Variant ForTypeEqualityCorrectness := .
+
+Lemma typeEqualityCorrectness
+      {T} `{FunctorLaws T}
+      {typeEqualityForT :
+         forall R,
+           ProgramAlgebra ForTypeEquality T R (TypeEqualityResult T)}
+      `{PA : ! ProofAlgebra ForTypeEqualityCorrectness T
+                     (sig (UniversalPropertyP typeEqualityCorrectnessStatement))}
+      `{! WellFormedProofAlgebra PA}
+  : forall tau, typeEqualityCorrectnessStatement (proj1_sig tau) (proj2_sig tau).
+Proof.
+  move => tau.
+  apply (
+      proj2_sig
+        (Induction
+           (P := UniversalPropertyP typeEqualityCorrectnessStatement)
+           _
+           (proj2_sig tau)
+        )
+    ).
+Qed.
