Semantics/Dynamic/Bool.v
@@ -21,118 +21,125 @@ From ExtensibleCompiler.Theory Require Import UniversalProperty.
 
 Local Open Scope SubFunctor_scope.
 
-Definition eval__Bool
-           {V} `{FunctorLaws V}
-           `{! V supports Bool}
-  : forall {T}, MixinAlgebra Bool T (EvalResult V)
-  := fun _ rec '(MkBool b) env => boolean b.
+Section Bool.
 
-Global Instance Eval__Bool
-       {V} `{FunctorLaws V}
-       `{! V supports Bool}
-  : forall {T}, ProgramAlgebra Eval Bool T (EvalResult V)
-  := fun _ => {| programAlgebra := eval__Bool; |}.
+  Context
+    {V}
+    `{FunctorLaws V}
+    `{! V supports Bool}
+  .
 
-Inductive EvalP__Bool {E V}
-          `{FunctorLaws E} `{FunctorLaws V}
-          `{! E supports Bool}
-          `{! V supports Bool}
-          (EvalP__E : (WellFormedValue E * WellFormedValue V) -> Prop)
-  : (WellFormedValue E * WellFormedValue V) -> Prop
-  :=
-  | BoolValue : forall b, EvalP__Bool EvalP__E (boolean b, boolean b)
-.
+  Definition eval__Bool
+    : forall {T}, MixinAlgebra Bool T (EvalResult V)
+    := fun _ rec '(MkBool b) env => boolean b.
 
-Inductive WellTyped__Bool
-          {T E}
-          `{FunctorLaws T} `{FunctorLaws E}
-          `{! T supports BoolType}
-          `{! E supports Bool}
-          (WT : TypedExpr T E -> Prop) : TypedExpr T E -> Prop :=
-| WellTyped__boolean : forall t e b,
-    proj1_sig e = boolean__F b ->
-    proj1_sig t = boolType ->
-    WellTyped__Bool WT {| type := t; expr := e; |}
-.
+  Global Instance Eval__Bool
+    : forall {T}, ProgramAlgebra ForEval Bool T (EvalResult V)
+    := fun _ => {| programAlgebra := eval__Bool; |}.
 
-Global Instance IndexedFunctor_WellTyped__Bool
-       {T V}
-       `{FunctorLaws T} `{FunctorLaws V}
-       `{! T supports BoolType}
-       `{! V supports Bool}
-  : IndexedFunctor (TypedExpr T V) WellTyped__Bool.
-Proof.
-  constructor.
-  move => A B i IH [] [t UP__t] [e UP__e] b /= => Eq__e Eq__t.
-  move : Eq__t Eq__e UP__t UP__e => -> -> => UP__t UP__e.
-  econstructor => //.
-Qed.
+  Global Instance WF_Eval__Bool
+    : WellFormedMendlerAlgebra (fun _ => Eval__Bool).
+  Proof.
+    constructor.
+    move => T T' f rec [] b //.
+  Qed.
 
-Definition SoundnessStatement__Bool
-           {T E V}
-           `{FunctorLaws T} `{FunctorLaws E} `{FunctorLaws V}
-           `{! E supports Bool}
-           (WT : (TypedExpr T V -> Prop) -> TypedExpr T V -> Prop)
-           `{Eval__E   : forall {R}, ProgramAlgebra Eval   E R (EvalResult   V)}
-           `{TypeOf__E : forall {R}, ProgramAlgebra TypeOf E R (TypeOfResult T)}
-           (recEval   : UniversalPropertyF E -> EvalResult   V)
-           (recTypeOf : UniversalPropertyF E -> TypeOfResult T)
-  :=
-    (SoundnessStatement__EvalAlgebra WT
-                                   (eval__E   := fun _ => programAlgebra' Eval__E)
-                                   (typeOf__F := fun _ => programAlgebra' TypeOf__E)
-                                   recEval recTypeOf
-    ).
+  Context
+    {E}
+    `{FunctorLaws E}
+    `{! E supports Bool}
+    `{! WellFormedSubFunctor Bool E}
+  .
 
-Global Instance EvalSoundness__Bool
+  Inductive EvalRelation__Bool
+            (EvalRelation__E : (WellFormedValue E * WellFormedValue V) -> Prop)
+    : (WellFormedValue E * WellFormedValue V) -> Prop
+    :=
+    | BoolValue : forall b, EvalRelation__Bool EvalRelation__E (boolean b, boolean b)
+  .
 
-       {T}
-       `{FunctorLaws T}
-       `{! T supports BoolType}
+  Context
+    {T}
+    `{FunctorLaws T}
+    `{! T supports BoolType}
+  .
 
-       {E}
-       `{FunctorLaws E}
-       `{! E supports Bool}
-       `{! WellFormedSubFunctor Bool E}
+  (* TODO: move this elsewhere *)
+  Inductive WellTyped__Bool
+            (WT : (TypedExpr T V)-indexedProp)
+    : (TypedExpr T V)-indexedProp
+    :=
+    | WellTyped__boolean : forall t e b,
+        proj1_sig e = boolean__F b ->
+        proj1_sig t = boolType ->
+        WellTyped__Bool WT {| type := t; expr := e; |}
+  .
 
-       {V}
-       `{FunctorLaws V}
-       `{! V supports Bool}
-
-       (WT : (TypedExpr T V -> Prop) -> TypedExpr T V -> Prop)
-       `(IndexedFunctor (TypedExpr T V) WT)
-       `((WellTyped__Bool <= WT)%IndexedSubFunctor)
-
-       `{Eval__E   : forall {R}, ProgramAlgebra Eval   E R (EvalResult   V)}
-       `{! forall {R}, WellFormedProgramAlgebra Eval__Bool Eval__E (T := R)}
-       (recEval   : UniversalPropertyF E -> EvalResult   V)
-
-       `{TypeOf__E : forall {R}, ProgramAlgebra TypeOf E R (TypeOfResult T)}
-       `{! forall {R}, WellFormedProgramAlgebra TypeOf__Bool TypeOf__E (T := R)}
-       (recTypeOf : UniversalPropertyF E -> TypeOfResult T)
-
-  : ProofAlgebra Bool (sig (UniversalPropertyP2 (SoundnessStatement__Bool WT recEval recTypeOf))).
-Proof.
-  constructor.
-  apply Induction2Algebra_Bool => b.
-  rewrite / SoundnessStatement__Bool / SoundnessStatement__EvalAlgebra / UniversalPropertyP2 /=.
-  constructor.
-  {
-    apply conj; apply (proj2_sig (boolean b)).
-  }
-  {
-    move => Gamma.
-    rewrite / boolean__F / boolean / inject /=.
-    rewrite unwrap__UP'_wrap__F /=.
-    rewrite fmapFusion / Extras.compose /=.
-    rewrite wellFormedSubFunctor => //=.
-    rewrite / programAlgebra'.
-    rewrite wellFormedProgramAlgebra.
-    rewrite wellFormedProgramAlgebra.
-    move => IH tau TY.
-    apply (iInject (F := WellTyped__Bool)) => /=.
+  Global Instance IndexedFunctor_WellTyped__Bool
+    : IndexedFunctor (TypedExpr T V) WellTyped__Bool.
+  Proof.
+    constructor.
+    move => A B i IH [] [t UP__t] [e UP__e] b /= => Eq__e Eq__t.
+    move : Eq__t Eq__e UP__t UP__e => -> -> => UP__t UP__e.
     econstructor => //.
-    move : TY => /=.
-    move => [] <- //.
-  }
+  Qed.
+
+  Global Instance Soundness__Bool
+
+         (WT : (TypedExpr T V)-indexedPropFunctor)
+         `(IndexedFunctor (TypedExpr T V) WT)
+         `((WellTyped__Bool <= WT)%IndexedSubFunctor)
+
+         `{Eval__E   : forall {R}, ProgramAlgebra ForEval   E R (EvalResult   V)}
+         `{! forall {R}, WellFormedProgramAlgebra Eval__Bool Eval__E (T := R)}
+         (recEval   : UniversalPropertyF E -> EvalResult   V)
+
+         `{TypeOf__E : forall {R}, ProgramAlgebra ForTypeOf E R (TypeOfResult T)}
+         `{! forall {R}, WellFormedProgramAlgebra TypeOf__Bool TypeOf__E (T := R)}
+         (recTypeOf : UniversalPropertyF E -> TypeOfResult T)
+
+    : ProofAlgebra
+        ForSoundness Bool
+        (sig (UniversalPropertyP2
+                (AbstractSoundnessStatement' WT recEval recTypeOf))).
+  Proof.
+    constructor.
+    apply Induction2Algebra_Bool => b.
+    rewrite / AbstractSoundnessStatement' / AbstractSoundnessStatement.
+    rewrite / UniversalPropertyP2 /=.
+    constructor.
+    {
+      apply conj; apply (proj2_sig (boolean b)).
+    }
+    {
+      move => Gamma.
+      rewrite / boolean__F / boolean / inject /=.
+      rewrite unwrap__UP'_wrap__F /=.
+      rewrite fmapFusion / Extras.compose /=.
+      rewrite wellFormedSubFunctor => //=.
+      rewrite / programAlgebra'.
+      rewrite wellFormedProgramAlgebra.
+      rewrite wellFormedProgramAlgebra.
+      move => IH tau TY.
+      apply (iInject (F := WellTyped__Bool)) => /=.
+      econstructor => //.
+      move : TY => /=.
+      move => [] <- //.
+    }
+  Qed.
+
+End Bool.
+
+(* small sanity check *)
+Definition Soundness__Bool'
+           {V}
+           `{FunctorLaws V}
+           `{! V supports Bool}
+           {T}
+           `{FunctorLaws T}
+           `{! T supports BoolType}
+  : Soundness__ProofAlgebra (T := T) (E := Bool) (V := V) WellTyped__Bool.
+Proof.
+  move => recEval recTypeOf.
+  apply : Soundness__Bool.
 Qed.
