Semantics/Dynamic/Lambda.v
@@ -14,51 +14,60 @@ From ExtensibleCompiler.Theory Require Import UniversalProperty.
 
 Local Open Scope SubFunctor_scope.
 
-Definition eval__Lambda
-           {LT L} `{FunctorLaws LT}
-           `{F : forall V, Functor (L V)} `{FL : forall V, FunctorLaws (L V)}
-           `{(L nat) supports (Closure L)}
-           `{(L nat) supports Stuck}
-  : MixinAlgebra (Lambda LT nat) (ValueFix (L nat)) (EvalResult (L nat))
-  := fun rec e env =>
-       match e with
-       | App f a =>
-         let f' := rec f env in
-         match isClosure (proj1_sig f') with
-         | Some (f, env') => rec f (insert (rec a env) env')
-         | None           => stuck "Non-function in call position"
-         end
-       | Lam v b => stuck "TODO"
-       | Var v   =>
-         match lookup env v with
-         | Some w => w
-         | None   => stuck "Variable lookup failed"
-         end
-       end.
+Section Lambda.
 
-Global Instance EvalAlgebra__Lambda
-       {LT L} `{FunctorLaws LT}
-       `{F : forall V, Functor (L V)} `{FL : forall V, FunctorLaws (L V)}
-       `{(L nat) supports (Closure L)}
-       `{(L nat) supports Stuck}
-  : ProgramAlgebra Eval (Lambda LT nat) (ValueFix (L nat)) (EvalResult (L nat))
-  := {| programAlgebra := eval__Lambda; |}.
+  Context
 
-(* TODO *)
+    {T}
+    `{FunctorLaws T}
 
-(* Inductive Eval__Lambda *)
-(*        {LT L} `{FunctorLaws LT} *)
-(*        `{F : forall V, Functor (L V)} `{FL : forall V, FunctorLaws (L V)} *)
-(*        `{(L nat) supports (Closure L)} *)
-(*        `{(L nat) supports Stuck} *)
-(*   : (WellFormedValue L * WellFormedValue V) -> Prop *)
-(*   := *)
-(*   | LambdaTrue : forall c t e t', *)
-(*       Eval (c, boolean true) -> *)
-(*       Eval (t, t') -> *)
-(*       Eval__Lambda Eval (lambda c t e, t') *)
-(*   | Lambdaalse : forall c t e e', *)
-(*       Eval (c, boolean false) -> *)
-(*       Eval (e, e') -> *)
-(*       Eval__Lambda Eval (lambda c t e, e') *)
-(* . *)
+    {E}
+    `{! forall Var, Functor (E Var)}
+    `{! forall Var, FunctorLaws (E Var)}
+    `{(E nat) supports (Closure E)}
+    `{(E nat) supports Stuck}
+
+  .
+
+  Definition eval__Lambda
+    : MixinAlgebra (Lambda T nat) (ValueFix (E nat)) (EvalResult (E nat))
+    := fun rec e env =>
+         match e with
+         | App f a =>
+           let f' := rec f env in
+           match isClosure (proj1_sig f') with
+           | Some (f, env') => rec f (insert (rec a env) env')
+           | None           => stuck "Non-function in call position"
+           end
+         | Lam v b => stuck "TODO"
+         | Var v   =>
+           match lookup env v with
+           | Some w => w
+           | None   => stuck "Variable lookup failed"
+           end
+         end.
+
+  Global Instance EvalAlgebra__Lambda
+    : ProgramAlgebra ForEval (Lambda T nat) (ValueFix (E nat)) (EvalResult (E nat))
+    := {| programAlgebra := eval__Lambda; |}.
+
+  (* TODO *)
+
+  (* Inductive Eval__Lambda *)
+  (*        {LT L} `{FunctorLaws LT} *)
+  (*        `{F : forall V, Functor (L V)} `{FL : forall V, FunctorLaws (L V)} *)
+  (*        `{(L nat) supports (Closure L)} *)
+  (*        `{(L nat) supports Stuck} *)
+  (*   : (WellFormedValue L * WellFormedValue V) -> Prop *)
+  (*   := *)
+  (*   | LambdaTrue : forall c t e t', *)
+  (*       Eval (c, boolean true) -> *)
+  (*       Eval (t, t') -> *)
+  (*       Eval__Lambda Eval (lambda c t e, t') *)
+  (*   | Lambdaalse : forall c t e e', *)
+  (*       Eval (c, boolean false) -> *)
+  (*       Eval (e, e') -> *)
+  (*       Eval__Lambda Eval (lambda c t e, e') *)
+  (* . *)
+
+End Lambda.
