Syntax/Types/BoolType.v
@@ -3,6 +3,7 @@ From Coq Require Import ssreflect.
 From ExtensibleCompiler.Theory Require Import Algebra.
 From ExtensibleCompiler.Theory Require Import Eval.
 From ExtensibleCompiler.Theory Require Import Functor.
+From ExtensibleCompiler.Theory Require Import ProofAlgebra.
 From ExtensibleCompiler.Theory Require Import ProgramAlgebra.
 From ExtensibleCompiler.Theory Require Import SubFunctor.
 From ExtensibleCompiler.Theory Require Import Sum1.
@@ -58,6 +59,49 @@ Definition typeEquality__BoolType
   := fun _ rec '(MkBoolType) => fun t => isBoolType (proj1_sig t).
 
 Global Instance TypeEquality__BoolType
-       LT `{FunctorLaws LT} `{LT supports BoolType}
-  : forall {T}, ProgramAlgebra TypeEquality BoolType T (TypeEqualityResult LT)
+       {LT} `{FunctorLaws LT} `{LT supports BoolType}
+  : forall {T}, ProgramAlgebra ForTypeEquality BoolType T (TypeEqualityResult LT)
   := fun _ => {| programAlgebra := typeEquality__BoolType |}.
+
+Global Instance TypeEqualityCorrectness__BoolType
+       T `{FunctorLaws T} `{! T supports BoolType}
+       `{! WellFormedSubFunctor BoolType T}
+       `{PA : forall {R}, ProgramAlgebra ForTypeEquality T R (TypeEqualityResult T)}
+       `{! forall {R}, WellFormedProgramAlgebra (T := R) TypeEquality__BoolType PA}
+  : ProofAlgebra
+      ForTypeEqualityCorrectness
+      BoolType
+      (sig (UniversalPropertyP (typeEqualityCorrectnessStatement (T := T)))).
+Proof.
+  constructor => [] [].
+  exists boolType.
+  rewrite / UniversalPropertyP.
+  econstructor.
+  rewrite / typeEqualityCorrectnessStatement.
+  move => tau'.
+  rewrite / typeEquality / mendlerFold {1} / boolType / boolType'.
+  rewrite {1} / inject /=.
+  rewrite {1} wellFormedSubFunctor /=.
+  rewrite {1} / wrap__F.
+  rewrite wellFormedProgramAlgebra /=.
+  rewrite / isBoolType.
+  case P : (project (proj1_sig tau')) => [ [] | ] // => _.
+  move : P.
+  rewrite / project.
+  move => P.
+  move : P (inj_prj _ _ P) => _.
+  rewrite / boolType / boolType' /=.
+  rewrite wellFormedSubFunctor /=.
+  move => P.
+  move : P (f_equal wrap__UP' P) => _.
+  move => P.
+  move : P (f_equal (@proj1_sig _ _) P) => _.
+  setoid_rewrite wrap__UP'_unwrap__UP'.
+  {
+    move => -> /=.
+    rewrite wellFormedSubFunctor //.
+  }
+  {
+    apply proj2_sig.
+  }
+Qed.
